reflecting existential variables, the_cancel_simplifier doesn't work anymore.

examples/AutoSep.v
@@ -57,6 +57,7 @@ Ltac the_cancel_simplifier :=
       Expr.Eq
       EquivDec.nat_eq_eqdec
       Provers.inSameGroup Provers.eqD Provers.eqD_seq Provers.transitivityEqProver
+
       Provers.groupsOf
       Provers.addEquality
       Provers.in_seq_dec
@@ -73,6 +74,7 @@ Ltac the_cancel_simplifier :=
       SepTac.SEP.sheapD SepTac.SEP.sexprD
       SepTac.SEP.starred SepTac.SEP.himp
       Expr.Impl
+
       Expr.is_well_typed 
     ].
 
@@ -80,9 +82,40 @@ Ltac vcgen :=
   structured_auto; autorewrite with sepFormula in *; simpl in *;
     unfold starB, hvarB, hpropB in *; fold hprop in *.
 
-Ltac sep := sym_eval ltac:isConst idtac unfolder (CORRECTNESS ptsto_evaluator) tt tt tt;
+Ltac sep := 
+  sym_eval ltac:isConst idtac unfolder (CORRECTNESS ptsto_evaluator) tt tt tt;
   repeat (ho;
     match goal with
-      | [ |- interp _ (![ _ ] _) ] => sep_canceler ltac:(isConst) idtac the_cancel_simplifier tt
+      | [ |- interp _ (![ _ ] _) ] => 
+        sep_canceler ltac:(isConst) (@Provers.transitivityEqProver) the_cancel_simplifier tt
       | _ => autorewrite with sepFormula; unfold substH; simpl; try congruence
     end).
+
+(*
+Definition readS : assert := st ~> ExX, Ex v, ![ $0 =*> v * #0 ] st
+  /\ st#Rp @@ (st' ~> [| st'#Rv = v |] /\ ![ $0 =*> v * #1 ] st').
+
+Definition read := bmodule "read" {{
+  bfunction "read" [readS] {
+    Rv <- $[0];;
+    If (Rv = 0) {
+      $[0] <- 0
+    } else {
+      $[0] <- 0
+    } ;;
+    Rv <- $[0];;
+    Goto Rp
+  }
+}}.
+
+Theorem readOk : moduleOk read.
+  vcgen. 
+  Focus 7.
+  sym_eval ltac:isConst idtac unfolder (CORRECTNESS ptsto_evaluator) tt tt tt.
+  ho. congruence.
+  autorewrite with sepFormula; unfold substH; simpl; try congruence.
+  sep_canceler ltac:(isConst) (@Provers.transitivityEqProverRec) the_cancel_simplifier tt.
+  
+  Set Printing Depth 70.
+  the_cancel_simplifier.
+*)
