src/SymIL.v
@@ -880,13 +880,15 @@ Qed.
     end.
   Ltac reflect_loc isConst l types funcs uvars vars k :=
     match l with
-      | Reg ?r => constr:(@SymReg types r)
+      | Reg ?r => 
+        let res := constr:(@SymReg types r) in
+        k uvars funcs res
       | Imm ?i =>
-        reflect_expr isConst i types funcs uvars vars ltac:(fun funcs i =>
-          let l := constr:(@SymImm types i) in k funcs l)
+        reflect_expr isConst i types funcs uvars vars ltac:(fun uvars funcs i =>
+          let l := constr:(@SymImm types i) in k uvars funcs l)
       | Indir ?r ?i =>
-        reflect_expr isConst i types funcs uvars vars ltac:(fun funcs i =>
-          let l := constr:(@SymIndir types r i) in k funcs l)
+        reflect_expr isConst i types funcs uvars vars ltac:(fun uvars funcs i =>
+          let l := constr:(@SymIndir types r i) in k uvars funcs l)
     end.
 
   Ltac collectTypes_lvalue isConst l Ts :=
@@ -896,10 +898,10 @@ Qed.
     end.
   Ltac reflect_lvalue isConst l types funcs uvars vars k :=
     match l with
-      | LvReg ?r => let l := constr:(@SymLvReg types r) in k funcs l 
+      | LvReg ?r => let l := constr:(@SymLvReg types r) in k uvars funcs l 
       | LvMem ?l => 
-        reflect_loc isConst l types funcs uvars vars ltac:(fun funcs l =>
-          let l := constr:(@SymLvMem types l) in k funcs l)
+        reflect_loc isConst l types funcs uvars vars ltac:(fun uvars funcs l =>
+          let l := constr:(@SymLvMem types l) in k uvars funcs l)
     end.
 
   Ltac collectTypes_rvalue isConst r Ts :=
@@ -912,13 +914,13 @@ Qed.
   Ltac reflect_rvalue isConst r types funcs uvars vars k :=
     match r with
       | RvLval ?l =>
-        reflect_lvalue isConst l types funcs uvars vars ltac:(fun funcs l =>
-          let l := constr:(@SymRvLval types l) in k funcs l)
+        reflect_lvalue isConst l types funcs uvars vars ltac:(fun uvars funcs l =>
+          let l := constr:(@SymRvLval types l) in k uvars funcs l)
       | RvImm ?i =>
-        reflect_expr isConst i types funcs uvars vars ltac:(fun funcs i =>
-          let l := constr:(@SymRvImm types i) in k funcs l)
+        reflect_expr isConst i types funcs uvars vars ltac:(fun uvars funcs i =>
+          let l := constr:(@SymRvImm types i) in k uvars funcs l)
       | RvLabel ?l => 
-        let r := constr:(@SymRvLabel types l) in k funcs r
+        let r := constr:(@SymRvLabel types l) in k uvars funcs r
     end.
 
   Ltac collectTypes_instr isConst i Ts :=
@@ -934,14 +936,14 @@ Qed.
   Ltac reflect_instr isConst i types funcs uvars vars k :=
     match i with
       | Assign ?l ?r =>
-        reflect_lvalue isConst l types funcs uvars vars ltac:(fun funcs l =>
-        reflect_rvalue isConst r types funcs uvars vars ltac:(fun funcs r =>
-          let res := constr:(@SymAssign types l r) in k funcs res))
+        reflect_lvalue isConst l types funcs uvars vars ltac:(fun uvars funcs l =>
+        reflect_rvalue isConst r types funcs uvars vars ltac:(fun uvars funcs r =>
+          let res := constr:(@SymAssign types l r) in k uvars funcs res))
       | Binop ?l ?r1 ?o ?r2 =>
-        reflect_lvalue isConst l types funcs uvars vars ltac:(fun funcs l =>
-        reflect_rvalue isConst r1 types funcs uvars vars ltac:(fun funcs r1 =>
-        reflect_rvalue isConst r2 types funcs uvars vars ltac:(fun funcs r2 =>
-          let res := constr:(@SymBinop types l r1 o r2) in k funcs res)))
+        reflect_lvalue isConst l types funcs uvars vars ltac:(fun uvars funcs l =>
+        reflect_rvalue isConst r1 types funcs uvars vars ltac:(fun uvars funcs r1 =>
+        reflect_rvalue isConst r2 types funcs uvars vars ltac:(fun uvars funcs r2 =>
+          let res := constr:(@SymBinop types l r1 o r2) in k uvars funcs res)))
     end.
 
   Ltac collectTypes_instrs isConst is Ts :=
@@ -954,11 +956,11 @@ Qed.
   Ltac reflect_instrs isConst is types funcs uvars vars k :=
     match is with
       | nil => 
-        let is := constr:(@nil (sym_instr types)) in k funcs is
+        let is := constr:(@nil (sym_instr types)) in k uvars funcs is
       | ?i :: ?is =>
-        reflect_instr isConst i types funcs uvars vars ltac:(fun funcs i =>
-        reflect_instrs isConst is types funcs uvars vars ltac:(fun funcs is =>
-          let res := constr:(i :: is) in k funcs res))
+        reflect_instr isConst i types funcs uvars vars ltac:(fun uvars funcs i =>
+        reflect_instrs isConst is types funcs uvars vars ltac:(fun uvars funcs is =>
+          let res := constr:(i :: is) in k uvars funcs res))
     end.
 
   Ltac isConst e :=
@@ -1087,14 +1089,18 @@ Qed.
                 match find_reg st Rv with
                   | (?rv_v, ?rv_pf) =>
                     let all_instrs := get_instrs st tt in
+                    let all_props := Expr.collect_props shouldReflect in
+                    let pures := Expr.props_types all_props in
+
                     let regs := constr:((rp_v, (sp_v, (rv_v, tt)))) in
                     (** collect the raw types **)
                     let Ts := collectAllTypes_instrs all_instrs Ts in
-                    let Ts := Expr.collectAllTypes_expr ltac:(isConst) Ts regs in
+                    let Ts := Expr.collectTypes_exprs ltac:(isConst) regs Ts in
+                    let Ts := Expr.collectTypes_exprs ltac:(isConst) pures Ts in
                     let Ts := SEP.collectAllTypes_sexpr isConst Ts (SF :: nil) in
                     let Ts := Expr.collectAllTypes_funcs Ts Fs in
                     let Ts := SEP.collectAllTypes_sfuncs Ts SFs in
-                    let Ts := Expr.collectAllTypes_props shouldReflect isConst Ts in
+(*                    let Ts := Expr.collectAllTypes_props shouldReflect isConst Ts in *)
                     (** check for potential universe problems **)
                     match Ts with
                       | context [ PropX.PropX ] => 
@@ -1124,38 +1130,39 @@ Qed.
                     let sfuncs := constr:(@nil (@SEP.ssignature typesV pcT stT)) in
                     let sfuncs := SEP.getAllSFunctions pcT stT typesV sfuncs SFs in
                     (** reflect the expressions **)
-                    let rec build_path instrs last funcs k :=
+                    let rec build_path instrs last uvars funcs k :=
                       match instrs with
-                        | tt => k funcs last
+                        | tt => k uvars funcs last
                         | ((?i, ?H), ?is) =>
                           match type of H with
                             | Structured.evalCond ?l ?t ?r _ ?st = _ =>
-                              reflect_rvalue ltac:(isConst) l typesV funcs uvars vars ltac:(fun funcs' l =>
-                              reflect_rvalue ltac:(isConst) r typesV funcs' uvars vars ltac:(fun funcs' r =>
+                              reflect_rvalue ltac:(isConst) l typesV funcs uvars vars ltac:(fun uvars funcs' l =>
+                              reflect_rvalue ltac:(isConst) r typesV funcs' uvars vars ltac:(fun uvars funcs' r =>
                                 let funcs_ext := Reflect.extension funcs funcs' in
                                 eapply (@evalPath_cond_app types_extV funcs funcs_ext uvars vars l t r _ _ _ _ last) in H;
                                 cbv iota in H ;
                                 clear last ; 
-                                build_path is H funcs' k))
+                                build_path is H uvars funcs' k))
                             | evalInstrs _ ?st _ = _ =>
-                              reflect_instrs ltac:(isConst) i typesV funcs uvars vars ltac:(fun funcs' sis =>
+                              reflect_instrs ltac:(isConst) i typesV funcs uvars vars ltac:(fun uvars funcs' sis =>
                                 let funcs_ext := Reflect.extension funcs funcs' in
                                 eapply (@evalPath_instrs_app types_extV funcs funcs_ext uvars vars sis _ _ _ _ last) in H ; 
                                 clear last ;
-                                build_path is H funcs' k)
+                                build_path is H uvars funcs' k)
                           end
                       end
                     in
-                    Expr.reflect_props shouldReflect ltac:(isConst) typesV funcs uvars vars ltac:(fun funcs pures proofs =>
-                    Expr.reflect_expr ltac:(isConst) rp_v typesV funcs uvars vars ltac:(fun funcs rp_v =>
-                    Expr.reflect_expr ltac:(isConst) sp_v typesV funcs uvars vars ltac:(fun funcs sp_v =>
-                    Expr.reflect_expr ltac:(isConst) rv_v typesV funcs uvars vars ltac:(fun funcs rv_v =>
-                    SEP.reflect_sexpr ltac:(isConst) SF typesV funcs pcT stT sfuncs uvars vars ltac:(fun funcs sfuncs SF =>
+                    Expr.reflect_exprs ltac:(isConst) pures typesV funcs uvars vars ltac:(fun uvars funcs pures =>
+                    let proofs := Expr.props_proof all_props in
+                    Expr.reflect_expr ltac:(isConst) rp_v typesV funcs uvars vars ltac:(fun uvars funcs rp_v =>
+                    Expr.reflect_expr ltac:(isConst) sp_v typesV funcs uvars vars ltac:(fun uvars funcs sp_v =>
+                    Expr.reflect_expr ltac:(isConst) rv_v typesV funcs uvars vars ltac:(fun uvars funcs rv_v =>
+                    SEP.reflect_sexpr ltac:(isConst) SF typesV funcs pcT stT sfuncs uvars vars ltac:(fun uvars funcs sfuncs SF =>
                     generalize (@evalPath_nil types_extV funcs uvars vars stn st) ;
                     let starter := fresh in
                     intro starter ;
                     let funcs := eval simpl app in funcs in
-                    build_path all_instrs starter funcs ltac:(fun funcs path =>
+                    build_path all_instrs starter uvars funcs ltac:(fun uvars funcs path =>
                       match funcs with
                         | _ :: _ :: _ :: _ :: _ :: ?funcs_ext => idtac ;
                           apply (@stateD_proof types_ext funcs uvars vars sfuncs _ sp_v rv_v rp_v 
@@ -1163,68 +1170,6 @@ Qed.
                           apply (@sym_eval_any _ _ C types_ext funcs_ext sfuncs stn uvars vars _ _ _ path) in H' ;
                           clear path ;
                           (simplifier H' || fail 1000000 "simplifier failed!") ;
-(*
-                          (unfolder H' || fail 1000000 "unfolder failed!") ;
-                          cbv beta iota zeta delta
-                            [ sym_evalInstrs sym_evalInstr sym_evalLval sym_evalRval sym_evalLoc sym_evalStream sym_assertTest
-                              sym_setReg sym_getReg
-                              SepExpr.pures SepExpr.impures SepExpr.other
-                              SymMem SymRegs SymPures
-                              SEP.star_SHeap SEP.liftSHeap SEP.multimap_join 
-                              Expr.SemiDec_expr Expr.expr_seq_dec Expr.tvar_val_sdec Expr.Eq Expr.liftExpr
-                              app map nth_error value error fold_right
-                              DepList.hlist_hd DepList.hlist_tl DepList.seq_dec 
-                              SepExpr.FM.find SepExpr.FM.add SepExpr.FM.remove SepExpr.FM.map SepExpr.FM.empty SepExpr.FM.fold
-                              Compare_dec.lt_eq_lt_dec nat_rec nat_rect Peano_dec.eq_nat_dec sumbool_rec sumbool_rect
-                              EquivDec.equiv_dec EquivDec.nat_eq_eqdec
-                              f_equal 
-                              bedrock_funcs bedrock_types pcT stT tvWord
-                              fst snd
-                              FuncImage PredImage TypeImage
-                              Env.repr Env.updateAt SEP.substV
-
-                              (* remove [stateD] *)
-                              stateD Expr.exprD 
-                              Expr.applyD Expr.exprD Expr.Range Expr.Domain Expr.Denotation Expr.lookupAs
-                              SEP.sheapD SEP.starred SEP.sexprD
-                              Expr.AllProvable
-                              Expr.Provable
-                              EquivDec.equiv_dec Expr.EqDec_tvar Expr.tvar_rec Expr.tvar_rect 
-                              Logic.eq_sym eq_sym f_equal
-                              eq_rec_r eq_rect eq_rec
-                              nat_rec nat_rect
-                              sumbool_rec sumbool_rect
-                              Expr.tvarD types
-
-                              SEP.himp SEP.sexprD Expr.Impl 
-                              Expr.applyD Expr.exprD Expr.Range Expr.Domain Expr.Denotation 
-                              Expr.lookupAs
-                              tvTest
-                              SepExpr.SDenotation SepExpr.SDomain
-                              EquivDec.nat_eq_eqdec  
-                              tvWord SEP.sheapD SEP.sepCancel
-                              SepExpr.impures SepExpr.pures SepExpr.other
-                              SEP.star_SHeap SEP.unify_remove_all 
-                              SEP.multimap_join SEP.liftSHeap SEP.unify_remove SEP.starred 
-                              Expr.tvarD Expr.Eq
-
-                              SepExpr.FM.fold SepExpr.FM.find SepExpr.FM.add SepExpr.FM.empty 
-                              bedrock_types 
-                                
-                              Compare_dec.lt_eq_lt_dec Peano_dec.eq_nat_dec
-                              SepExpr.FM.map ExprUnify.exprUnifyArgs ExprUnify.empty_Subst
-                              ExprUnify.exprUnify ExprUnify.fold_left_2_opt 
-                              fold_right value error map nth_error app                                       
-                              pcT stT 
-                              EquivDec.equiv_dec Expr.EqDec_tvar Expr.tvar_rec Expr.tvar_rect 
-                              ExprUnify.get_Eq
-                              types
-                              Provers.transitivityProverRec Provers.transitivityEqProver Provers.inSameGroup
-                              Provers.in_seq_dec
-                              Provers.eqD Provers.eqD_seq
-                              Expr.typeof comparator
-                            ] in H' ; 
-*)
                           subst typesV; subst types_extV ;
                           (try assumption ||
                            destruct H' as [ [ ? [ ? ? ] ] [ ? ? ] ])
